@prefix owl: <http://www.w3.org/2002/07/owl#> .
@prefix rdf: <http://www.w3.org/1999/02/22-rdf-syntax-ns#> .
@prefix rdfs: <http://www.w3.org/2000/01/rdf-schema#> .
@prefix foaf: <http://xmlns.com/foaf/0.1/> .
@prefix xsd: <http://www.w3.org/2001/XMLSchema#> .
@prefix dcterms: <http://dublincore.org/2012/06/14/dcterms#> .
@prefix dcelements: <http://dublincore.org/2012/06/14/dcelements#> .
@prefix sec: <https://w3id.org/security#> .
@prefix vc: <https://w3id.org/credentials/v1#> .
@prefix svc: <http://dig.csail.mit.edu/2018/svc#> .

<http://dig.csail.mit.edu/2018/svc#> a owl:Ontology ;
    dcterms:title "The Solid Verifiable Credentials Schema Vocabulary"@en ;
    rdfs:comment """
    This ontology describes the classes and properties that are key
    to the SolidVC ecosystem. The design is intentionally terse and
    focused in order to allow for a relatively simple interface for
    the production and consumption of verifiable credentials.
    
    This ontology was developed by Kayode Ezike (kezike17@mit.edu)
    as a component of his MEng thesis work with DIG.
    """@en .

svc:Credential a rdfs:Class ;
    rdfs:isDefinedBy <http://dig.csail.mit.edu/2018/svc#> ;
    rdfs:subClassOf rdfs:Resource ;
    rdfs:label "Credential"@en ;
    rdfs:comment "The class representing a credential in the form of groups of statements and attestations about an entity"@en .

svc:id a rdf:Property ;
    rdfs:isDefinedBy <http://dig.csail.mit.edu/2018/svc#> ;
    rdfs:label "id"@en ;
    rdfs:comment "The ID (likely URI; may be superfluous) of a credential"@en ;
    rdfs:domain svc:Credential ;
    rdfs:range rdfs:Literal .

svc:plain a rdf:Property ;
    rdfs:isDefinedBy <http://dig.csail.mit.edu/2018/svc#> ;
    rdfs:label "plain"@en ;
    rdfs:comment "The plaintext RDF graph representing a credential"@en ;
    rdfs:domain svc:Credential ;
    rdfs:range rdfs:Resource .

svc:domain a rdf:Property ;
    rdfs:isDefinedBy <http://dig.csail.mit.edu/2018/svc#> ;
    rdfs:label "domain"@en ;
    rdfs:comment "The domain of a credential (e.g., 'HEALTH', 'LAW', 'TRAVEL', 'GENERAL')"@en ;
    rdfs:domain svc:Credential ;
    rdfs:range rdfs:Literal .

svc:title a rdf:Property ;
    rdfs:isDefinedBy <http://dig.csail.mit.edu/2018/svc#> ;
    rdfs:label "title"@en ;
    rdfs:comment "The title briefly describing a credential (e.g., 'MEng. Credential Request for Kayode Ezike')"@en ;
    rdfs:domain svc:Credential ;
    rdfs:range rdfs:Literal .

svc:description a rdf:Property ;
    rdfs:isDefinedBy <http://dig.csail.mit.edu/2018/svc#> ;
    rdfs:label "description"@en ;
    rdfs:comment "An optional description of a credential request"@en ;
    rdfs:domain svc:Credential ;
    rdfs:range rdfs:Literal .

svc:messageStatus a rdf:Property ;
    rdfs:isDefinedBy <http://dig.csail.mit.edu/2018/svc#> ;
    rdfs:label "messageStatus"@en ;
    rdfs:comment "Status of message (e.g., 'APPROVED', 'DECLINED')"@en ;
    rdfs:domain svc:Credential ;
    rdfs:range rdfs:Literal .

svc:messageType a rdf:Property ;
    rdfs:isDefinedBy <http://dig.csail.mit.edu/2018/svc#> ;
    rdfs:label "messageType"@en ;
    rdfs:comment "Type of message (e.g., 'REQUEST', 'ISSUANCE', 'ASSERTION', 'VERIFICATION', 'INQUIRY', 'MISCELLANEOUS')"@en ;
    rdfs:domain svc:Credential ;
    rdfs:range rdfs:Literal .
    
svc:issuerId a rdf:Property ;
    rdfs:isDefinedBy <http://dig.csail.mit.edu/2018/svc#> ;
    rdfs:label "issuerId"@en ;
    rdfs:comment "The ID of the issuer of a credential (e.g., 'https://kezike.solid.community/profile/card#me')"@en ;
    rdfs:domain svc:Credential ;
    rdfs:range rdfs:Literal .

svc:issuanceDate a rdf:Property ;
    rdfs:isDefinedBy <http://dig.csail.mit.edu/2018/svc#> ;
    rdfs:label "issuanceDate"@en ;
    rdfs:comment "The issuance date of a credential"@en ;
    rdfs:domain svc:Credential ;
    rdfs:range xsd:dateTime .

svc:subjectId a rdf:Property ;
    rdfs:isDefinedBy <http://dig.csail.mit.edu/2018/svc#> ;
    rdfs:label "subjectId"@en ;
    rdfs:comment "The ID of the subject of a credential (e.g., 'https://kezike.solid.community/profile/card#me')"@en ;
    rdfs:domain svc:Credential ;
    rdfs:range rdfs:Literal .

svc:publicKey a rdf:Property ;
    rdfs:isDefinedBy <http://dig.csail.mit.edu/2018/svc#> ;
    rdfs:label "publicKey"@en ;
    rdfs:comment "The URI of the public key of the subject of a credential (similar to sec:publicKey)"@en ;
    rdfs:domain foaf:PersonalProfileDocument ;
    rdfs:range rdfs:Literal .

svc:revocationList a rdf:Property ;
    rdfs:isDefinedBy <http://dig.csail.mit.edu/2018/svc#> ;
    rdfs:label "revocationList"@en ;
    rdfs:comment "The URI of the revocation list of a user (similar to vc:credentialStatus)"@en ;
    rdfs:domain foaf:PersonalProfileDocument ;
    rdfs:range rdfs:Literal .

svc:proof a rdf:Property ;
    rdfs:isDefinedBy <http://dig.csail.mit.edu/2018/svc#> ;
    rdfs:label "proof"@en ;
    rdfs:comment """
    The digital proof verifying a credential (similar to sec:proof):
    - 'type': The proof type (e.g., sec:RsaSignature2018)
    - 'created': The timestamp of the creation of a credential
    - 'creator': The public key of the issuer of a credential
    - 'nonce': Optional value proving effort in proof creation
    - 'signatureValue': The creator's signature of plain
    """@en ;
    rdfs:domain svc:Credential ;
    rdfs:range rdfs:Literal .

svc:CredentialStatusList a rdfs:Class ;
    rdfs:isDefinedBy <http://dig.csail.mit.edu/2018/svc#> ;
    rdfs:subClassOf svc:Credential ;
    rdfs:label "CredentialStatusList"@en ;
    rdfs:comment "The class representing a credential status in the form of groups of statements and attestations about a credential (similar to vc:CredentialStatusList2017)"@en .

svc:credentialStatus a rdf:Property ;
    rdfs:isDefinedBy <http://dig.csail.mit.edu/2018/svc#> ;
    rdfs:label "credentialStatus"@en ;
    rdfs:comment "Status of a credential (e.g., 'ACTIVE', 'EXPIRED', 'REVOKED')"@en ;
    rdfs:domain svc:CredentialStatusList ;
    rdfs:range rdfs:Literal .

svc:credentialId a rdf:Property ;
    rdfs:isDefinedBy <http://dig.csail.mit.edu/2018/svc#> ;
    rdfs:label "credentialId"@en ;
    rdfs:comment "ID of a credential"@en ;
    rdfs:domain svc:CredentialStatusList ;
    rdfs:range rdfs:Literal .

svc:revocationReason a rdf:Property ;
    rdfs:isDefinedBy <http://dig.csail.mit.edu/2018/svc#> ;
    rdfs:label "revocationReason"@en ;
    rdfs:comment "Reasoning behind credential revocation"@en ;
    rdfs:domain svc:CredentialStatusList ;
    rdfs:range rdfs:Literal .

svc:revocationDate a rdf:Property ;
    rdfs:isDefinedBy <http://dig.csail.mit.edu/2018/svc#> ;
    rdfs:label "revocationDate"@en ;
    rdfs:comment "Date of credential revocation"@en ;
    rdfs:domain svc:CredentialStatusList ;
    rdfs:range xsd:dateTime .
